last commit before deleting old stuff

src/birkhoff.lean
@@ -1,42 +1,38 @@
 /-birkhoof.lean -- Birkhoff's HSP Theorem in Lean
 
-  Notes:Recall, 
-        -`Prop` is syntactic sugar for `Sort 0`, the bottom of the type hierarchy.
-          Like the other type universes, it is closed under the arrow constructor 
-          (if `p q : Prop`, then `p → q : Prop`)
-        -`Type u` is syntactic sugar for `Sort (u+1)`
-          (`Prop = Type -1` and `Sort 1 = Type 0`)
+  Author: William DeMeo <williamdemeo@gmail.com>
+  Date: 26 Nov 2018
+
+  References
+  [1] Bergman, Clifford, "Universal algebra," CRC Press, 2012
+
+  Copyright: 2018 William DeMeo  (See the LICENSE file)
 -/
--- import basic
+
 import basic
 import subuniverse 
 import data.set
 
-section
+universe s -- where operation (s)ymbols live
+universe u -- where structure (u)niverses (i.e. carriers) live
+universe u' -- where structure (u)niverses (i.e. carriers) live
+universe u'' -- where structure (u)niverses (i.e. carriers) live
+universe a -- where (a)rities live
 
-  universe s -- where operation (s)ymbols live
-  universe u -- where structure (u)niverses (i.e. carriers) live
-  universe a -- where (a)rities live
+section
 
   parameter υ : Sort u  -- A carrier type
   parameter τ : Sort u  -- Another carrier type
 
-  -- Operation on the carrier υ (of arity α) 
   -- (defined in basic.lean)  def op (υ : Sort u) (α : Sort a) := (α → υ) → υ  
-
-  -- Restricted Operation on the carrier υ (of arity α) 
-  def op_restricted {υ : Sort u} (r : υ → Prop) (α : Sort a) := (α → (υ → Prop)) → (υ → Prop) 
-
   -- (defined in basic.lean) structure signature := mk :: (F : Sort s) (ρ : F → Sort a)
 
-  parameters {α : Type*} {β : Type*} {S : signature} (A : algebra_on S α) 
-  parameters (B : algebra_on S β) {I ζ : Type} {R : I → set α} 
+  parameters {S : signature}
   open set
   open subuniverse
-
   -- Elementary Facts ------------------------------------------
 
-  /- Lemma (cf. Ex. 1.16.6 of Bergman~\cite{MR2839398})
+  /- Lemma (cf. Ex. 1.16.6 of [1])
      Let $f$ and $g$ be homomorphisms from $\mathbf A$ to $\mathbf B$.
      Let $E(f,g) = \{ a \in A : f(a) = g(a) \}$ (the **equalizer** of $f$ and $g$). 
      1. $E(f,g)$ is a subuniverse of $\mathbf A$.
@@ -46,79 +42,274 @@ section
         $|Hom(\mathbf A, \mathbf B)| \leq |B|^{|X|}$. -/
 
   -- equalizer for generic functions
-  def equalizer (h : α → β) (g : α → β) : set α := λ (x : α), h x = g x 
+ --(A : algebra_on S α) (B : algebra_on S β) (C : algebra_on S γ) -- {I ζ : Type} {R : I → set α} 
+  def equalizer {α : Type u} {β : Type u'}
+  (h : α → β) (g : α → β) : set α := λ (x : α), h x = g x 
 
   -- indicates whether h is a homomorphism  
-  def hom (h : α → β) : Prop := ∀ f a, h (A f a) = B f (h ∘ a)
+  def hom_on {α : Type u} {β : Type u'} (A : algebra_on S α) (B : algebra_on S β) (h : α → β) 
+  : Prop := ∀ f a, h (A f a) = B f (h ∘ a)
 
-  def equalizer_of_homs (h : α → β) (g : α → β) 
-  (hh : hom h) (hg : hom g) : set α := λ a, h a = g a 
+  def hom {A : algebra S} {B : algebra S} (h : A → B) 
+  : Prop := ∀ f a, h (A f a) = B f (h ∘ a)
 
-  variables (h : α → β) (g : α → β)  (hh : hom h)  (hg : hom g) 
+
+  -- composition of homomorphisms is a homomorphism
+  lemma hom_comp_hom_of_hom {A : algebra S} {B : algebra S} {C : algebra S}
+  (h : A → B)  {h₁ : hom h} (g : B → C) {h₂ : hom g} : 
+  hom (g ∘ h) := assume f a, show (g ∘ h)(A f a) = C f (g ∘ h ∘ a), from 
+  have h₃ : (g ∘ h)(A f a) = g (h (A f a)), from  rfl,
+  calc (g ∘ h)(A f a) = g ((B f) (h ∘ a)) : (h₁ f a) ▸ h₃ 
+                  ... = (C f) (g ∘ h ∘ a) : h₂ f (h ∘ a)
+
+  -- composition of homomorphisms is a homomorphism
+  lemma hom_on_comp_hom_on_of_hom_on {α : Type u} {β : Type u'} {γ : Type u''}
+  {A : algebra_on S α} {B : algebra_on S β} {C : algebra_on S γ}
+  (h : α → β)  {h₁ : hom_on A B h} (g : β → γ) {h₂ : hom_on B C g} : 
+  hom_on A C (g ∘ h) := assume f a, show (g ∘ h)(A f a) = C f (g ∘ h ∘ a), from 
+  have h₃ : (g ∘ h)(A f a) = g (h (A f a)), from  rfl,
+  calc (g ∘ h)(A f a) = g ((B f) (h ∘ a)) : (h₁ f a) ▸ h₃ 
+                  ... = (C f) (g ∘ h ∘ a) : h₂ f (h ∘ a)
+  
+  
+  
+  -- the set on which two homs agree
+  def equalizer_of_homs {A : algebra S} {B : algebra S}
+  (h : A → B) (g : A → B) {hh : hom h} {hg : hom g} : set A := λ a, h a = g a 
+
+  -- the set on which two hom_on's agree
+  def equalizer_of_hom_on {α : Type u} {β : Type u'} {A : algebra_on S α} {B : algebra_on S β}
+  (h : α → β) (g : α → β) {hh : hom_on A B h} {hg : hom_on A B g} : set α := λ a, h a = g a 
+
 
   -- 1. The equalizer $E(f,g)$ is a subuniverse of $\mathbf A$.
-  lemma sub_equalizer (h : α → β) (g : α → β) (hh : hom h)  (hg : hom g) : 
-  Sub A (equalizer_of_homs h g hh hg) := 
-  assume f a (h₁: ∀ x, a x ∈ equalizer_of_homs h g hh hg),
-  show A f a ∈ (equalizer_of_homs h g hh hg),  from 
+  lemma sub_equalizer_of_homs {A : algebra S} {B : algebra S}
+  (h : A → B) (g : A → B) (hh : hom h)  (hg : hom g) : 
+  Sub A (equalizer h g) := 
+    assume f a (h₁: ∀ x, a x ∈ equalizer h g),
+    show A f a ∈ (equalizer h g),  from 
+      have h₂ : h ∘ a = g ∘ a, from funext h₁, 
+      show h (A f a) = g (A f a), from 
+        calc h (A f a) = (B f) (h ∘ a): hh f a
+                   ... = (B f) (g ∘ a): congr_arg (B f) h₂ 
+                   ... = g (A f a) : eq.symm (hg f a)
+
+  -- 1. The equalizer $E(f,g)$ is a subuniverse of $\mathbf A$.
+  lemma sub_equalizer_of_hom_on {α : Type u} {β : Type u'} {A : algebra_on S α} {B : algebra_on S β}
+  (h : α → β) (g : α → β) (hh : hom_on A B h)  (hg : hom_on A B g) : 
+  Sub A (equalizer h g) := 
+  assume f a (h₁: ∀ x, a x ∈ equalizer h g),
+  show A f a ∈ (equalizer h g),  from 
     have h₂ : h ∘ a = g ∘ a, from funext h₁, 
     show h (A f a) = g (A f a), from 
       calc h (A f a) = (B f) (h ∘ a): hh f a
                  ... = (B f) (g ∘ a): congr_arg (B f) h₂ 
                  ... = g (A f a) : eq.symm (hg f a)
+
   
 
   -- 2. If $X ⊆ A$, if $Sg(X) = \mathbf A$, and if $f x = g x$ for all $x ∈ X$, then $f = g$. 
 
-lemma mem_of_eq (s t : set α) : s = t →  ∀ x, x ∈ s → x ∈ t := 
-begin intros h x h', rw ←h, assumption end
+  lemma mem_of_eq {α : Type u} (s t : set α) : s = t →  ∀ x, x ∈ s → x ∈ t := 
+  begin intros h x h', rw ←h, assumption end
 
-lemma hom_determined_on_gens (h : α → β) (g : α → β)
-(hh : hom h) (hg : hom g) (X : set α) : 
-(∀ x, x ∈ X → h x = g x) → (∀ a, a ∈ Sg A X → h a = g a) := 
-assume (h₁ : ∀ x, x ∈ X → h x = g x), 
-assume a (h₂ : a ∈ Sg A X), show h a = g a, from 
-  have h₃ : a ∈ Y A X, from mem_of_eq (Sg A X) (Y A X) (sg_inductive A X) a h₂,
-  Y.rec 
-    --base step: assume a = x ∈ X
-    h₁ 
-    --inductive step: assume a = A f b for some b with ∀ i, b i ∈ Sg X
-    ( assume f b (h₄ : ∀ i, b i ∈ Y A X)  (h₅ : ∀ i, h (b i) = g (b i)),
-      show h (A f b) = g (A f b), from 
-      have h₆ : h ∘ b = g ∘ b, from funext h₅, 
-      calc h (A f b) = (B f) (h ∘ b) : hh f b
-                 ... = (B f) (g ∘ b) : congr_arg (B f) h₆    
-                 ... = g (A f b)     : eq.symm (hg f b)) h₃ 
+  lemma hom_determined_on_gens {A : algebra S} {B : algebra S}
+  (h : A → B) (g : A → B) (hh : hom h) (hg : hom g) (X : set A) : 
+  X ⊆ equalizer h g → Sg A X ⊆ equalizer h g := 
+  -- Idea of the proof: we have
+  --     1. X ⊆ equalizer h g,
+  --     2. Sub (equalizer h g), i.e., equalizer h g is a subalgebra
+  --     3. and Sg X is the smallest subalgebra containing X
+  -- Therefore, Sg X ⊆ equalizer h g, which means h = g on Sg X.
+  assume h₁ : X ⊆ equalizer h g, show Sg A X ⊆ equalizer h g, from 
+  assume a (h₂ : a ∈ Sg A X), show a ∈ equalizer h g, from 
+  have h₃ : Sub A (equalizer h g), from (sub_equalizer_of_homs h g hh hg),
+      (sInter_mem A a) h₂ h₃ h₁
 
--- A better proof would use sub_equalizer lemma, since we know 
--- 1. X ⊆ equalizer h g,
--- 2. Sub (equalizer h g), i.e., equalizer h g is a subalgebra
--- 3. and Sg X is the smallest subalgebra containing X
--- It follows that Sg X ⊆ equalizer h g, which means h = g on Sg X.
+  lemma hom_on_determined_on_gens {α : Type u} {β : Type u'} {A : algebra_on S α} {B : algebra_on S β}
+  (h : α → β) (g : α → β) (hh : hom_on A B h) (hg : hom_on A B g) (X : set α) : 
+  X ⊆ equalizer h g → Sg A X ⊆ equalizer h g := 
+  -- Idea of the proof: we have
+  --     1. X ⊆ equalizer h g,
+  --     2. Sub (equalizer h g), i.e., equalizer h g is a subalgebra
+  --     3. and Sg X is the smallest subalgebra containing X
+  -- Therefore, Sg X ⊆ equalizer h g, which means h = g on Sg X.
+  assume h₁ : X ⊆ equalizer h g, show Sg A X ⊆ equalizer h g, from 
+  assume a (h₂ : a ∈ Sg A X), show a ∈ equalizer h g, from 
+  have h₃ : Sub A (equalizer h g), from (sub_equalizer_of_hom_on h g hh hg),
+      (sInter_mem A a) h₂ h₃ h₁
+
+  -- Here's another proof of the last result using the recursor of Y.
+  lemma hom_determined_on_gens_rec {A : algebra S} {B : algebra S} 
+  (h : A → B) (g : A → B)  (hh : hom h) (hg : hom g) (X : set A) : 
+  (∀ x, x ∈ X → h x = g x) → (∀ a, a ∈ Sg A X → h a = g a) := 
+  assume (h₁ : ∀ x, x ∈ X → h x = g x), 
+  assume a (h₂ : a ∈ Sg A X), show h a = g a, from 
+    have h₃ : a ∈ Y A X, from mem_of_eq (Sg A X) (Y A X) (sg_inductive A X) a h₂,
+    Y.rec 
+      --base step: assume a = x ∈ X
+      h₁ 
+      --inductive step: assume a = A f b for some b with ∀ i, b i ∈ Sg X
+      ( assume f b (h₄ : ∀ i, b i ∈ Y A X)  (h₅ : ∀ i, h (b i) = g (b i)),
+        show h (A f b) = g (A f b), from 
+        have h₆ : h ∘ b = g ∘ b, from funext h₅, 
+        calc h (A f b) = (B f) (h ∘ b) : hh f b
+                   ... = (B f) (g ∘ b) : congr_arg (B f) h₆    
+                   ... = g (A f b)     : eq.symm (hg f b)) h₃ 
 
 
 
- /- 
-  Suppose the subset $X \subseteq A$ generates $\mathbf A$ and suppose
-  $f |_X = g |_X$.
-  Fix an arbitrary element $a\in A$.  We show $f(a) = g(a)$.
-  Since $X$ generates $\mathbf A$, there exists a (say, $n$-ary) term $t$ and 
-  a tuple $(x_1, \dots, x_n) \in X^n$ such that 
-  $a = t^{\mathbf A}(x_1, \dots, x_n)$. Therefore, 
-  \begin{align*}
-    f(a) = f(t^{\mathbf A}(x_1, \dots, x_n)) &= t^{\mathbf B}(f(x_1), \dots, f(x_n))\\
-                                    &= t^{\mathbf B}(g(x_1), \dots, g(x_n))
-                                     = g(t^{\mathbf A}(x_1, \dots, x_n)) = g(a).
-  \end{align*}
-  In other words, a homomorphism is uniquely determined by its restriction to 
-  a generating set.
-  -/
+  -- def surjective {α : Type u} {β : Type u'} (f : α → β ) : Prop := ∀ y, ∃ x, f x = y
+  --  def injective {α : Type u} {β : Type u'} (f : α → β) : Prop := ∀ ⦃x₁ x₂⦄, f x₁ = f x₂ → x₁ = x₂
+    -- def bijective {α : Type u} {β : Type u'} (f : α → β) : Prop := injective f ∧ surjective f
 
-/-  
+  open classical function
+  local attribute [instance] prop_decidable
+
+  noncomputable def inverse' {α : Type u} {β : Type u'} (f : α → β) (default : α)  : β → α :=
+  λ b, if h : ∃ a, f a = b then some h else default
+
+  -- The right inverse of a surjective function.
+  noncomputable def right_inv {α : Type u} {β : Type u'} (f : α → β)
+  (h₁ : surjective f) : β → α := λ b, some (h₁ b)
+
+  -- A surjective function has a right inverse.
+  lemma right_inv_is_right_inverse {α : Type u} {β : Type u'} (f : α → β) 
+  (h₁ : surjective f) : ∀ b, b = f ((right_inv f h₁) b) := 
+  assume b, have h₂ : (right_inv f h₁) b = some (h₁ b), from rfl,
+  have h₃ : f (some (h₁ b)) = b, from some_spec (h₁ b),
+  eq.subst (eq.symm h₂) (eq.symm h₃)
+
+  -- Right inverse of an epimorphism is a homomorphism.
+  lemma right_inv_of_epi_is_hom {A : algebra S} {B : algebra S} (g : A → B) 
+  (h₁ : surjective g) (h₂ : hom g) : hom (right_inv g h₁) := 
+  let g_inv := (right_inv g h₁) in 
+  show hom g_inv, from 
+  assume f b, show g_inv (B f b) = A f (g_inv ∘ b), from  sorry
+
+  -- Right inverse of an epimorphism is a homomorphism.
+  lemma right_inv_of_epi_is_hom_on {α : Type u} {β : Type u'} 
+  {A : algebra_on S α} {B : algebra_on S β} (g : α → β) 
+  (h₁ : surjective g) (h₂ : hom_on A B g) : hom_on B A (right_inv g h₁) := 
+  let g_inv := (right_inv g h₁) in 
+  show hom_on B A g_inv, from 
+  assume f b, show g_inv (B f b) = A f (g_inv ∘ b), from  sorry
+
   
-   There are exactly $|B|^{|X|}$ functions from $X$ to $B$ so, 
-  assuming $X$ generates $\mathbf A$, we have
-  $|Hom(\mathbf A,\mathbf B)| \leq |B|^{|X|}$.
-  -/
+  def ker {α : Type u} {β : Type u'} (f : α → β) : α → α → Prop := λ a b, f a = f b
 
+  /-Lemma (Ex. 1.26.8.a. [1])
+    Suppose $f ∈ Hom(A,B)$, $g ∈ Hom(A,C)$, $h$ is surjective, and $ker f ⊆ ker g$. 
+    Then, $∃ h ∈ Hom(B, C)$ such that $g = h ∘ f$.
+ 
+    If $f : A → B$ is epi
+       $g : A → C$ is hom
+       $ker f ⊆ ker g$
+    Then $∃ h : B → C$ with $g = h ∘ f$ and $h$ is a homomorphism.
+  -/
+  lemma hom_on_facotor_down {α : Type u} {β : Type u'} {γ : Type u''}
+  {A : algebra_on S α} {B : algebra_on S β} {C : algebra_on S γ} 
+  (f : α → β) (hf : hom_on A B f) (hs : surjective f) 
+  (g : α → γ) (hg : hom_on A C g) 
+  (kk : ∀ a b, ker f a b → ker g a b) : ∃ h : β → γ, (g = h ∘ f) ∧ (hom_on B C h) := 
+  let h := g ∘ (right_inv f hs)  in 
+  have h₁ : hom_on B C h, from sorry,
+  have h₃ : g = h ∘ f, from sorry, 
+  exists.intro h (and.intro h₃ h₁) 
+
+  lemma hom_facotor_down {A : algebra S} {B : algebra S} {C : algebra S} 
+  -- assumptions:
+  (f : A → B) (hf : hom f) (hs : surjective f)    -- f is epi
+  (g : A → C) (hg : hom g)                        -- g is hom
+  (kk : ∀ a b, ker f a b → ker g a b) :           -- ker f ⊆ ker g
+  -- conclusion:
+  ∃ h : B → C, (g = h ∘ f) ∧ (hom h) := 
+  -- proof:
+  let h := g ∘ (right_inv f hs)  in 
+    have h₁ : hom h, from sorry,
+    have h₃ : g = h ∘ f, from sorry, 
+    exists.intro h (and.intro h₃ h₁) 
+  /-
+       A---f----> B
+       |        /
+       g       h
+       |     /
+       |   /
+       V L
+       C
+  -/
+ 
+
+  /-Lemma (Ex. 1.26.8.b) [1])
+    Let $f : A → B$ and $g : A → C$ be homomorphisms, with $g$ surjective. 
+    If $ker g ⊆ ker f$, then there is a homomorphism $h : C → B$ st $f = h ∘ g$.
+  
+    If $f : A → B$ is hom
+       $g : A → C$ is epi
+       $ker g ⊆ ker f$
+    Then $∃ h : B → C$ with $f = h ∘ g$ and $h$ is a homomorphism.
+  -/
+  lemma hom_facotor_up {A : algebra S} {B : algebra S} {C : algebra S} 
+  -- assumptions:
+  (f : A → B) (hf : hom f)                        -- f is hom
+  (g : A → C) (hg : hom g) (hs : surjective g)    -- g is epi
+  (kk : ∀ a b, ker g a b → ker f a b) :           -- ker g ⊆ ker f
+  -- conclusion:
+  ∃ h : C → B,  (f = h ∘ g) ∧ (hom h) := 
+  -- proof:
+  let h := f ∘ (right_inv g hs)  in 
+    have h₁ : hom h, from sorry,
+    have h₃ : f = h ∘ g, from sorry, 
+    exists.intro h (and.intro h₃ h₁) 
+  
+  
+  lemma hom_on_facotor_up {α : Type u} {β : Type u'} {γ : Type u''}
+  {A : algebra_on S α} {B : algebra_on S β} {C : algebra_on S γ} 
+  (f : α → β) (hf : hom_on A B f) 
+  (g : α → γ) (hg : hom_on A C g) (hs : surjective g) 
+  (kk : ∀ a b, ker g a b → ker f a b) : ∃ h : γ → β,  (f = h ∘ g) ∧ (hom_on C B h) := 
+  let h := f ∘ (right_inv g hs)  in 
+  have h₁ : hom_on C B h, from sorry,
+  have h₃ : f = h ∘ g, from sorry, 
+  exists.intro h (and.intro h₃ h₁) 
+  /-
+       A----f----> B
+       |         7
+       g       /
+       |     h
+       |   /
+       V /
+       C
+ -/
+ 
 end                                                                                                                                                                                                                                            
+
+
+/- Miscellaneous Notes  
+
+Recall, 
+  - `Prop` is syntactic sugar for `Sort 0`, the bottom of the type hierarchy.
+    Like the other type universes, it is closed under the arrow constructor 
+    (if `p q : Prop`, then `p → q : Prop`)
+  -`Type u` is syntactic sugar for `Sort (u+1)`
+    (`Prop = Type -1` and `Sort 1 = Type 0`)
+
+
+-/
+/-
+Refereces:
+[1] @book {MR2839398,
+    AUTHOR = {Bergman, Clifford},
+     TITLE = {Universal algebra},
+    SERIES = {Pure and Applied Mathematics (Boca Raton)},
+    VOLUME = {301},
+      NOTE = {Fundamentals and selected topics},
+ PUBLISHER = {CRC Press, Boca Raton, FL},
+      YEAR = {2012},
+     PAGES = {xii+308},
+      ISBN = {978-1-4398-5129-6},
+   MRCLASS = {08-02 (06-02 08A40 08B05 08B10 08B26)},
+  MRNUMBER = {2839398 (2012k:08001)},
+MRREVIEWER = {Konrad P. Pi{\'o}ro},
+}
+-/
